add cinv lemmata and start simple automation

IrisCore/AuthHeap.thy
@@ -3,6 +3,10 @@ imports DerivedConstructions Frac BaseLogicShallow Misc
 begin
 
 subsubsection \<open>View based heap\<close>
+
+text \<open>Unique name for singleton heap camera\<close>
+definition "heap_name :: gname \<equiv> 0"
+
 type_synonym ('l,'v) heap = "('l,'v) map_view"
 
 lemma heap_auth_agree:
@@ -35,7 +39,7 @@ proof -
   qed
 qed
 
-lemma heap_frag_valid: "\<V>(constr_heap (\<circle>V [k\<mapsto>(dq,to_ag v)])) \<turnstile> \<upharpoonleft>(valid dq)"
+lemma heap_frag_valid: "\<V>(constr_heap \<gamma> (\<circle>V [k\<mapsto>(dq,to_ag v)])) \<turnstile> \<upharpoonleft>(valid dq)"
   by transfer' 
   (auto simp: constr_heap_def prod_n_valid_def \<epsilon>_n_valid view_frag_def valid_raw_map_view.rep_eq 
     map_view_rel_def split: option.splits)
@@ -46,22 +50,22 @@ lemma heap_op: "[l\<mapsto>(dq1, to_ag v1)]\<cdot>[l\<mapsto>(dq2, to_ag v2)] = 
 lemma heap_op_val_eq: "[l\<mapsto>(dq1, to_ag v)]\<cdot>[l\<mapsto>(dq2, to_ag v)] = [l\<mapsto>(dq1\<cdot>dq2, to_ag v)]" 
   unfolding heap_op by (auto simp: op_prod_def op_ag_def to_ag_def Rep_ag_inverse)
 
-lemma iprop_heap_valid: "\<V>(constr_heap h) \<turnstile> \<V>(h::heap_lang_heap)"
+lemma iprop_heap_valid: "\<V>(constr_heap \<gamma> h) \<turnstile> \<V>(h::heap_lang_heap)"
   apply (simp add: upred_valid_def upred_entails.rep_eq Abs_upred_f_inverse constr_heap_def)
   using prod_n_valid_snd[OF prod_n_valid_snd[OF prod_n_valid_snd[OF prod_n_valid_snd[OF prod_n_valid_snd]]]] 
   by fastforce
 
 text \<open>Heap camera operations\<close>
 abbreviation own_heap :: "heap_lang_heap \<Rightarrow> iprop" ("Own\<^sub>h _") where
-   "own_heap h \<equiv> Own(constr_heap h)"
+   "own_heap h \<equiv> Own(constr_heap heap_name h)"
 
 definition own_heap_auth :: "frac \<Rightarrow> (loc,val option) fmap \<Rightarrow> iprop" where
   "own_heap_auth q m \<equiv> Own\<^sub>h(map_view_auth (DfracOwn q) m)"
-
+  
 text \<open>Because our heap camera does not contain meta tokens, this proposition is just about owning a heap.\<close>
 definition heap_interp :: "(loc,val option) fmap \<Rightarrow> iprop" where
   "heap_interp \<sigma> \<equiv> own_heap_auth 1 \<sigma>" 
-  
+ 
 definition points_to :: "loc \<Rightarrow> dfrac \<Rightarrow> val \<Rightarrow> iprop" where
   "points_to l dq v = Own\<^sub>h(map_view_frag l dq (Some v))"
 abbreviation points_to_disc :: "loc \<Rightarrow> val \<Rightarrow> iprop" where 
@@ -70,22 +74,20 @@ abbreviation points_to_own :: "loc \<Rightarrow> frac \<Rightarrow> val \<Righta
   "points_to_own \<equiv> \<lambda>l p v. points_to l (DfracOwn p) v"
 abbreviation points_to_full :: "loc \<Rightarrow> val \<Rightarrow> iprop" where
   "points_to_full \<equiv> \<lambda>l v. points_to_own l 1 v"
+  
+notation points_to ("_ \<mapsto>{_} _" 60)
+notation points_to_disc (infix "\<mapsto>\<box>" 60)
+notation points_to_own ("_\<mapsto>{#_}_" 60)
+notation points_to_full (infix "\<mapsto>\<^sub>u" 60)
 
-bundle points_to_syntax begin
-  notation points_to ("_ \<mapsto>{_} _" 60)
-  notation points_to_disc (infix "\<mapsto>\<box>" 60)
-  notation points_to_own ("_\<mapsto>{#_}_" 60)
-  notation points_to_full (infix "\<mapsto>\<^sub>u" 60)
-end
-
-context includes points_to_syntax assumes "SORT_CONSTRAINT('c::ucamera)" begin 
+context assumes "SORT_CONSTRAINT('c::ucamera)" begin 
 
 lemma points_to_valid: 
   "(l \<mapsto>{dq} v) -\<^emph> \<upharpoonleft>(valid dq)"
 proof -
-  have "(l \<mapsto>{dq} v) \<turnstile> \<V>(constr_heap (\<circle>V [l\<mapsto>(dq,to_ag (Some v))]))" 
+  have "(l \<mapsto>{dq} v) \<turnstile> \<V>(constr_heap heap_name (\<circle>V [l\<mapsto>(dq,to_ag (Some v))]))" 
     by (auto simp: points_to_def own_valid map_view_frag_def)
-  moreover have "\<V>(constr_heap (\<circle>V [l\<mapsto>(dq,to_ag (Some v))])) \<turnstile> 
+  moreover have "\<V>(constr_heap heap_name (\<circle>V [l\<mapsto>(dq,to_ag (Some v))])) \<turnstile> 
     \<V>((\<circle>V [l\<mapsto>(dq,to_ag (Some v))])::heap_lang_heap)"
     using iprop_heap_valid by blast
   ultimately have "(l \<mapsto>{dq} v) \<turnstile> \<upharpoonleft>(valid dq)"
@@ -96,10 +98,11 @@ qed
 lemma points_to_agree: "upred_holds ((l \<mapsto>{dq1} v1) -\<^emph> ((l \<mapsto>{dq2} v2) -\<^emph> \<upharpoonleft>(v1 = v2)))"
 proof -
   have "upred_holds ((l \<mapsto>{dq1} v1) -\<^emph> ((l \<mapsto>{dq2} v2)) -\<^emph> 
-    \<V>(constr_heap (\<circle>V [l\<mapsto>(dq1, to_ag (Some v1))]) \<cdot> constr_heap (\<circle>V [l\<mapsto>(dq2, to_ag (Some v2))])))"
+    \<V>(constr_heap heap_name (\<circle>V [l\<mapsto>(dq1, to_ag (Some v1))]) \<cdot> 
+    constr_heap heap_name (\<circle>V [l\<mapsto>(dq2, to_ag (Some v2))])))"
     apply (simp add: points_to_def) using own_valid2 by (metis map_view_frag_def)
   then have "upred_holds ((l \<mapsto>{dq1} v1) -\<^emph> ((l \<mapsto>{dq2} v2)) -\<^emph> 
-    \<V>(constr_heap (\<circle>V ([l\<mapsto>(dq1, to_ag (Some v1))\<cdot>(dq2, to_ag (Some v2))]))))"
+    \<V>(constr_heap heap_name (\<circle>V ([l\<mapsto>(dq1, to_ag (Some v1))\<cdot>(dq2, to_ag (Some v2))]))))"
     apply (simp add: \<epsilon>_left_id op_prod_def constr_heap_def op_map_view_def map_view_auth_proj_def
       \<epsilon>_map_view_def map_view_frag_proj_def view_frag_def heap_op)
     by (auto simp: op_option_def)   
@@ -141,17 +144,21 @@ lemma points_to_frac_ne:
   shows "upred_holds ((l1 \<mapsto>{dq1} v1) -\<^emph> ((l2 \<mapsto>{dq2} v2) -\<^emph> \<upharpoonleft>(l1\<noteq>l2)))"
 proof -
   have valid_drop : 
-    "valid (constr_heap (\<circle>V [l1\<mapsto>(dq1,to_ag (Some v1))]) \<cdot> constr_heap (\<circle>V [l2\<mapsto>(dq2,to_ag (Some v2))])) =
+    "valid (constr_heap heap_name (\<circle>V [l1\<mapsto>(dq1,to_ag (Some v1))]) \<cdot> 
+    constr_heap heap_name (\<circle>V [l2\<mapsto>(dq2,to_ag (Some v2))])) =
       valid ((\<circle>V [l1\<mapsto>(dq1,to_ag (Some v1))]) \<cdot> (\<circle>V [l2\<mapsto>(dq2,to_ag (Some v2))]))"
     by (simp add: op_prod_def \<epsilon>_left_id \<epsilon>_valid prod_valid_def constr_heap_def)
-  have "\<V>((constr_heap (\<circle>V [l1\<mapsto>(dq1,to_ag (Some v1))]) \<cdot> constr_heap (\<circle>V [l2\<mapsto>(dq2,to_ag (Some v2))]))) 
-    \<turnstile> \<upharpoonleft>(valid (constr_heap (\<circle>V [l1\<mapsto>(dq1,to_ag (Some v1))]) \<cdot> constr_heap (\<circle>V [l2\<mapsto>(dq2,to_ag (Some v2))])))"
+  have "\<V>((constr_heap heap_name (\<circle>V [l1\<mapsto>(dq1,to_ag (Some v1))]) \<cdot> 
+      constr_heap heap_name (\<circle>V [l2\<mapsto>(dq2,to_ag (Some v2))]))) 
+    \<turnstile> \<upharpoonleft>(valid (constr_heap heap_name (\<circle>V [l1\<mapsto>(dq1,to_ag (Some v1))]) \<cdot> 
+      constr_heap heap_name (\<circle>V [l2\<mapsto>(dq2,to_ag (Some v2))])))"
     apply (simp add: op_prod_def \<epsilon>_left_id constr_heap_def)
     apply (simp add: upred_pure.rep_eq upred_entails.rep_eq upred_valid.rep_eq)
     apply (simp add: prod_n_valid_fun_def prod_valid_def \<epsilon>_valid \<epsilon>_n_valid)
     using dcamera_valid_iff by auto
   then have base: "upred_holds ((l1 \<mapsto>{dq1} v1) -\<^emph> ((l2 \<mapsto>{dq2} v2)) -\<^emph> 
-    \<upharpoonleft>(valid (constr_heap (\<circle>V [l1\<mapsto>(dq1,to_ag (Some v1))]) \<cdot> constr_heap (\<circle>V [l2\<mapsto>(dq2,to_ag (Some v2))]))))"
+    \<upharpoonleft>(valid (constr_heap heap_name (\<circle>V [l1\<mapsto>(dq1,to_ag (Some v1))]) \<cdot> 
+    constr_heap heap_name (\<circle>V [l2\<mapsto>(dq2,to_ag (Some v2))]))))"
     using upred_wand_holds2I[OF upred_entails_trans[OF upred_wand_holds2E[OF own_valid2]]] points_to_def
     by (smt (verit) map_view_frag_def)
   from assms have "valid ((\<circle>V [l1\<mapsto>(dq1,to_ag (Some v1))]) \<cdot> (\<circle>V [l2\<mapsto>(dq2,to_ag (Some v2))])) 
@@ -164,7 +171,8 @@ proof -
   then have "\<upharpoonleft>(valid ((\<circle>V [l1\<mapsto>(dq1,to_ag (Some v1))]) \<cdot> (\<circle>V [l2\<mapsto>(dq2,to_ag (Some v2))]))) \<turnstile>
     \<upharpoonleft>(l1\<noteq>l2)" using pure_entailsI by blast
   with valid_drop have 
-    "\<upharpoonleft>(valid (constr_heap (\<circle>V [l1\<mapsto>(dq1,to_ag (Some v1))]) \<cdot> constr_heap (\<circle>V [l2\<mapsto>(dq2,to_ag (Some v2))]))) 
+    "\<upharpoonleft>(valid (constr_heap heap_name (\<circle>V [l1\<mapsto>(dq1,to_ag (Some v1))]) \<cdot> 
+    constr_heap heap_name (\<circle>V [l2\<mapsto>(dq2,to_ag (Some v2))]))) 
     \<turnstile> \<upharpoonleft>(l1\<noteq>l2)" by simp
     from upred_entails_wand_holdsR2[OF this base] show ?thesis .
 qed
@@ -175,8 +183,12 @@ by (rule points_to_frac_ne[OF dfrac_not_valid_own])
 end
 
 subsubsection \<open>Prophecy map camera\<close>
+
+text \<open>Unique name for singleton proph_map camera\<close>
+definition "proph_map_name :: gname \<equiv> 4"
+
 abbreviation proph_own :: "heap_lang_proph_map \<Rightarrow> iprop" ("Own\<^sub>p _") where
-  "proph_own pm \<equiv> Own(constr_proph pm)"
+  "proph_own pm \<equiv> Own(constr_proph proph_map_name pm)"
 
 abbreviation own_proph_auth :: "frac \<Rightarrow> heap_lang_proph_map_raw \<Rightarrow> iprop" where
   "own_proph_auth q m \<equiv> Own\<^sub>p(map_view_auth (DfracOwn q) m)" 
